Rename Framing modules into regular Steel modules

ulib/experimental/Steel.Primitive.ForkJoin.fst
@@ -21,13 +21,11 @@ module L = Steel.SpinLock
 open Steel.FractionalPermission
 open FStar.Ghost
 open Steel.Reference
-open Steel.SteelT.Basics
+//open Steel.SteelT.Basics
 
 //module U = FStar.Universe
 
 ////////////////////////////////////////////////////////////////////////////////
-
-let full = full_perm
 
 let maybe_p (p:slprop) (v:bool) = if v then p else emp
 
@@ -46,87 +44,103 @@ type thread (p:slprop u#1) = {
   l:L.lock (lock_inv r p)
 }
 
+// From basics
+assume
+val drop (p:slprop) : SteelT unit p (fun _ -> emp)
+
+assume val intro_exists (#a:Type) (x:a) (p:a -> slprop)
+  : SteelT unit (p x) (fun _ -> h_exists p)
+
+assume
+val change_slprop
+  (p q:slprop)
+  (proof: (m:mem) -> Lemma (requires interp p m) (ensures interp q m))
+  : SteelT unit p (fun _ -> q)
+
+assume
+val par (#preL:slprop) (#postL:unit -> slprop)
+        ($f:unit -> SteelT unit preL postL)
+        (#preR:slprop) (#postR:unit -> slprop)
+        ($g:unit -> SteelT unit preR postR)
+  : SteelT unit
+    (preL `star` preR)
+    (fun x -> postL () `star` postR ())
+
+assume
+val cond (#a:Type) (b:bool) (p: bool -> slprop) (q: bool -> a -> slprop)
+         (then_: (unit -> SteelT a (p true) (q true)))
+         (else_: (unit -> SteelT a (p false) (q false)))
+  : SteelT a (p b) (q b)
+
+
 let intro_maybe_p_false (p:slprop)
   : SteelT unit emp (fun _ -> maybe_p p false)
-  = h_assert (maybe_p p false)
+  = change_slprop emp (maybe_p p false) (fun _ -> ())
 
 let intro_maybe_p_true (p:slprop)
   : SteelT unit p (fun _ -> maybe_p p true)
-  = h_assert (maybe_p p true)
+  = change_slprop p (maybe_p p true) (fun _ -> ())
+
+let intro_lock_inv_pred (r:ref bool) (p:slprop) (v:bool)
+  : SteelT unit
+      (pts_to r full_perm v `star` maybe_p p v)
+      (fun _ -> lock_inv_pred r p v)
+  = change_slprop (pts_to r full_perm v `star` maybe_p p v) (lock_inv_pred r p v) (fun _ -> ())
+
 
 let new_thread (p:slprop)
   : SteelT (thread p) emp (fun _ -> emp)
-  = intro_maybe_p_false p;
-    h_assert (maybe_p p false);
-    h_intro_emp_l (maybe_p p false);
-    let r = frame #(ref bool) #emp #(fun r -> pts_to r full_perm false)
-                  (fun () -> alloc false)
-                  (maybe_p p false) in
-    intro_h_exists false (lock_inv_pred r p);
-    let l  = L.new_lock (lock_inv r p) in
-    let t  =  { r = r ; l = l } in
-    return t
+  = let r = alloc false in
+    change_slprop (pts_to r full_perm false `star` emp) (lock_inv_pred r p false) (fun _ -> ());
+    intro_exists false (lock_inv_pred r p);
+    let l = L.new_lock (lock_inv r p) in
+    let t = {r = r; l = l} in
+    t
 
 let finish (#p:slprop) (t:thread p) (v:bool)
-  : SteelT unit (pts_to t.r full v `star` p) (fun _ -> emp)
-  = frame (fun _ -> write t.r true) p;
-    h_assert (pts_to t.r full true `star` p);
-    h_commute (pts_to t.r full true) p;
-    frame (fun _ -> intro_maybe_p_true p) (pts_to t.r full true);
-    h_commute (maybe_p p true) (pts_to t.r full true);
-    intro_h_exists true (lock_inv_pred t.r p);
+  : SteelT unit (pts_to t.r full_perm v `star` p) (fun _ -> emp)
+  = write t.r true;
+    change_slprop (pts_to t.r full_perm true `star` p) (lock_inv_pred t.r p true) (fun _ -> ());
+    intro_exists true (lock_inv_pred t.r p);
     L.release t.l
 
+
 let acquire (#p:slprop) (t:thread p)
-  : SteelT bool emp (fun b -> pts_to t.r full b)
+  : SteelT bool emp (fun b -> pts_to t.r full_perm b)
   = L.acquire t.l;
-    let b = read_refine (maybe_p p) t.r in
-    h_affine (pts_to t.r full b) (maybe_p p b);
-    return b
+    let b = read_refine #_ #full_perm (maybe_p p) t.r in
+    drop (maybe_p p b);
+    b
 
 let spawn (#p #q:slprop)
           ($f: (unit -> SteelT unit p (fun _ -> q)))
           (t:thread q)
           (_:unit)
   : SteelT unit p (fun _ -> emp)
-  = h_intro_emp_l p;
-    let b  = frame (fun () -> acquire t) p in
-    h_commute (pts_to t.r full b) p;
-    let _ = frame f (pts_to t.r full b) in
-    h_commute q (pts_to t.r full b);
+  = let b = acquire t in
+    f ();
     finish t b
 
 let fork (#p #q #r #s:slprop)
       (f: (unit -> SteelT unit p (fun _ -> q)))
       (g: (thread q -> unit -> SteelT unit r (fun _ -> s)))
   : SteelT unit (p `star` r) (fun _ -> s)
-  = h_intro_emp_l (p `star` r);
-    let t : thread q = frame (fun _ -> new_thread q) (p `star` r) in
-    h_assert (emp `star` (p `star` r));
-    h_elim_emp_l (p `star` r);
-    par (spawn f t) (g t);
-    h_elim_emp_l s
-
-let pre (#p:slprop) (t:thread p) (b:bool) : slprop = lock_inv_pred t.r p b
-let post (p:slprop) (b:bool) (_:unit) : slprop = p
+  = let t : thread q = new_thread q in
+    par (spawn f t) (g t)
 
 let join_case_true (#p:slprop) (t:thread p) (_:unit)
-  : SteelT unit (pre t true) (post p true)
-  = h_commute _ (maybe_p p true);
-    h_assert (maybe_p p true `star` pts_to t.r full true);
-    h_affine (maybe_p p true) (pts_to t.r full true);
-    h_assert (maybe_p p true)
+  : SteelT unit (lock_inv_pred t.r p true) (fun _ -> p)
+  = change_slprop (lock_inv_pred t.r p true) p (fun _ -> ())
 
-let join_case_false (#p:slprop) (t:thread p) (loop: (t:thread p -> SteelT unit emp (fun _ -> p))) (_:unit)
-  : SteelT unit (pre t false) (post p false)
-  = intro_h_exists false (lock_inv_pred t.r p);
+let join_case_false (#p:slprop) (t:thread p)
+  (loop: (t:thread p -> SteelT unit emp (fun _ -> p))) (_:unit)
+  : SteelT unit (lock_inv_pred t.r p false) (fun _ -> p)
+  = intro_exists false (lock_inv_pred t.r p);
     L.release t.l;
     loop t
 
 let rec join (#p:slprop) (t:thread p)
   : SteelT unit emp (fun _ -> p)
-  = L.acquire t.l;
-    let b = read_refine (maybe_p p) t.r in
-    h_assert (pts_to t.r full b `star` maybe_p p b);
-    h_assert (pre t b);
-    cond b (pre t) (post p) (join_case_true t) (join_case_false t (join #p))
+  = let _ = L.acquire t.l in
+    let b = read_refine #_ #full_perm (maybe_p p) t.r in
+    cond b (lock_inv_pred t.r p) (fun _ _ -> p) (join_case_true t) (join_case_false t join)
